barrier/parameter.v
@@ -1,0 +1,5 @@
+Require Export barrier.heap_lang.
+Require Import iris.parameter.
+
+Definition Σ := IParamConst heap_lang unitRA.
+Print Assumptions Σ.
